theories/Validity/Irrelevance.v
@@ -28,7 +28,7 @@ Proof.
     specialize (ih _ VΓad').
     intros; split; intros []; unshelve econstructor.
     1,2: now eapply ih.
-    all: now eapply SirrLR.
+    all: now eapply irrLR.
 Qed.
 
 Succeed Constraint u1 < v1.
@@ -65,14 +65,16 @@ Proof.
     destruct x as [lA'[ VΓ'' [VA' ->]]].
     intros ????? [tleq hdeq].
     pose (tleq' := IHVΓ VΓ'' _ wfΔ wfΔ' _ _ tleq).
-    exists tleq'; now eapply symLR, SirrLR.
+    exists tleq'.
+    symmetry; eapply irrLRCum, hdeq.
+    now eapply validTyExt, tleq.
 Qed.
 
 Lemma symValidTy {Γ Γ' l A B} {VΓ : [||-v Γ ≅ Γ']} (VΓ' : [||-v Γ' ≅ Γ]) :
-  [Γ ||-vS<l> A ≅ B | VΓ] -> [Γ' ||-vS<l> B ≅ A | VΓ'].
+  [Γ ||-v<l> A ≅ B | VΓ] -> [Γ' ||-v<l> B ≅ A | VΓ'].
 Proof.
   intros; constructor; intros; symmetry.
-  now unshelve (eapply (SvalidTyExt (Γ:=Γ) (Γ':=Γ')); tea; now eapply symSubst).
+  now unshelve (eapply (validTyExt (Γ:=Γ) (Γ':=Γ')); tea; now eapply symSubst).
 Qed.
 
 Lemma symValid {Γ Γ'} : [||-v Γ ≅ Γ'] -> [||-v Γ' ≅ Γ].
@@ -94,7 +96,7 @@ Proof.
     intros []; now constructor.
   - intros * ih *. pose proof (invValidity VΓ0) as (?&?&?&?&?&e&h); subst; cbn in h; subst.
     intros [tl hd]; pose proof (tl' := ih _ _ _ _ _ _ tl).
-    exists tl'; now eapply SirrLREqCum.
+    exists tl'; now eapply irrLREqCum.
 Qed.
 
 Lemma convSubst' {Γ Γ' Γ''}
@@ -109,14 +111,15 @@ Qed.
 
 Lemma convValidTy {Γ Γ' Γ''}
   (VΓ' : [||-v Γ ≅ Γ']) (VΓ'' : [||-v Γ ≅ Γ'']) {l A B} :
-  [_ ||-vS<l> A ≅ B | VΓ'] -> [_ ||-vS<l> A ≅ B | VΓ''].
-Proof. intros VA; constructor. intros. eapply (SvalidTyExt (Γ:=Γ) (Γ':=Γ')); tea; now eapply convSubst.
-  Unshelve.
+  [_ ||-v<l> A ≅ B | VΓ'] -> [_ ||-v<l> A ≅ B | VΓ''].
+Proof.
+  intros VA; constructor; intros.
+  eapply (validTyExt (Γ:=Γ) (Γ':=Γ')); tea; now eapply convSubst.
 Qed.
 
 Lemma convValidTy' {Γ Γ' Γ''}
   (VΓ : [||-v Γ ≅ Γ']) (VΓ' : [||-v Γ'' ≅ Γ']) {l A B} :
-  [_ ||-vS<l> A ≅ B | VΓ] -> [_ ||-vS<l> A ≅ B | VΓ'].
+  [_ ||-v<l> A ≅ B | VΓ] -> [_ ||-v<l> A ≅ B | VΓ'].
 Proof.
   intros ?%(symValidTy (symValid VΓ)).
   unshelve now eapply symValidTy, convValidTy.
@@ -139,16 +142,16 @@ Proof.
     intros VΓ'; pose proof (invValiditySnoc VΓ') as (?&?&?&?); subst.
     intros ???? wfΔ [tl hd] [tl' hd'].
     pose (tl'' := ih _ _ _ _ _ _ _ _ tl tl').
-    exists tl''; etransitivity; [now eapply SirrLR|].
-    eapply SirrLRCum; tea; symmetry; now eapply SvalidTyExt.
+    exists tl''; etransitivity; [now eapply irrLR|].
+    eapply irrLRCum; tea; symmetry; now eapply validTyExt.
 Qed.
 
 Lemma ureflValidTy {Γ Γ' l A B} (VΓ : [||-v Γ ≅ Γ']) (VΓ' : [||-v Γ' ≅ Γ']) :
-  [Γ ||-vS<l> A ≅ B | VΓ] -> [Γ' ||-vS<l> B ≅ B | VΓ'].
+  [Γ ||-v<l> A ≅ B | VΓ] -> [Γ' ||-v<l> B ≅ B | VΓ'].
 Proof.
   constructor; intros; etransitivity.
-  2: eapply SvalidTyExt; tea; now eapply convSubst'.
-  symmetry; eapply SvalidTyExt; tea.
+  2: eapply validTyExt; tea; now eapply convSubst'.
+  symmetry; eapply validTyExt; tea.
   unshelve eapply convSubst'; [| tea|].
   unshelve (eapply transSubst; tea; now eapply symSubst); tea.
 Qed.
@@ -161,10 +164,10 @@ Proof.
 Qed.
 
 Lemma irrLvlValidTy {Γ Γ' l l' A B C} (VΓ : [||-v Γ ≅ Γ']) :
-  [Γ ||-vS<l> A ≅ B | VΓ ] -> [Γ ||-vS<l'> B ≅ C | VΓ] -> [Γ ||-vS<l> B ≅ C | VΓ].
+  [Γ ||-v<l> A ≅ B | VΓ ] -> [Γ ||-v<l'> B ≅ C | VΓ] -> [Γ ||-v<l> B ≅ C | VΓ].
 Proof.
   constructor; intros.
-  eapply transLR; [eapply urefl|];  eapply SvalidTyExt; tea.
+  eapply transLR; [eapply urefl|]; eapply validTyExt; tea.
   unshelve (eapply transSubst; [|eapply convSubst, symSubst]; tea).
   2: now eapply symValid.
   now eapply ureflValid.
@@ -172,9 +175,9 @@ Qed.
 
 Lemma transValidTy {Γ Γ' Γ'' l l' A B C}
   (VΓ : [||-v Γ ≅ Γ']) (VΓ' : [||-v Γ' ≅ Γ'']) (VΓ'' : [||-v Γ ≅ Γ'']) :
-  [Γ ||-vS<l> A ≅ B | VΓ ] -> [Γ' ||-vS<l'> B ≅ C | VΓ'] -> [Γ ||-vS<l> A ≅ C | VΓ''].
+  [Γ ||-v<l> A ≅ B | VΓ ] -> [Γ' ||-v<l'> B ≅ C | VΓ'] -> [Γ ||-v<l> A ≅ C | VΓ''].
 Proof.
-  constructor; intros; etransitivity; eapply SvalidTyExt; tea.
+  constructor; intros; etransitivity; eapply validTyExt; tea.
   2: eapply irrLvlValidTy; [now eapply convValidTy|now eapply convValidTy'].
   eapply transSubst; tea.
   unshelve now eapply convSubst, symSubst.
@@ -208,7 +211,7 @@ Proof.
     now eapply urefl.
 Qed.
 
-Instance perValidTy {Γ Γ' l} (VΓ : [||-v Γ ≅ Γ']) : PER (StypeValidity _ _ VΓ l).
+Instance perValidTy {Γ Γ' l} (VΓ : [||-v Γ ≅ Γ']) : PER (typeValidity _ _ VΓ l).
 Proof.
   constructor; red; intros.
   - unshelve now eapply symValidTy, convValidTy, convValidTy'.
@@ -217,7 +220,7 @@ Proof.
     now eapply urefl.
 Qed.
 
-Instance iperValidTy l : IPER (VAdequate VR) (fun _ => term) (fun _ _ VΓ => StypeValidity _ _ VΓ l).
+Instance iperValidTy l : IPER (VAdequate VR) (fun _ => term) (fun _ _ VΓ => typeValidity _ _ VΓ l).
 Proof.
   constructor.
   - intros; now eapply symValidTy.
@@ -237,7 +240,7 @@ Qed.
 Lemma irrValidTy  {Γ0 Γ0' Γ1 Γ1' l A B}
   {VΓ0 : [||-v Γ0 ≅ Γ0']}
   {VΓ1 : [||-v Γ1 ≅ Γ1']}
-  : [||-v Γ0 ≅ Γ1] -> [Γ0 ||-vS<l> A ≅ B | VΓ0] -> [Γ1 ||-vS<l> A ≅ B | VΓ1].
+  : [||-v Γ0 ≅ Γ1] -> [Γ0 ||-v<l> A ≅ B | VΓ0] -> [Γ1 ||-v<l> A ≅ B | VΓ1].
 Proof.
   intros; unshelve now eapply convValidTy, convValidTy'.
   etransitivity; [|tea]; now symmetry.
@@ -245,22 +248,22 @@ Qed.
 
 Lemma irrValidTyRfl {Γ Γ' l A B}
   {VΓ VΓ' : [||-v Γ ≅ Γ']}
-  : [Γ ||-vS<l> A ≅ B | VΓ] -> [Γ ||-vS<l> A ≅ B | VΓ'].
+  : [Γ ||-v<l> A ≅ B | VΓ] -> [Γ ||-v<l> A ≅ B | VΓ'].
 Proof.
   eapply irrValidTy; now eapply lrefl.
 Qed.
 
 Lemma symValidTy' {Γ Γ' l A B} {VΓ : [||-v Γ ≅ Γ']} :
-  [_ ||-vS<l> A ≅ B | VΓ] -> [_ ||-vS<l> B ≅ A | symValid VΓ].
+  [_ ||-v<l> A ≅ B | VΓ] -> [_ ||-v<l> B ≅ A | symValid VΓ].
 Proof. eapply symValidTy. Qed.
 
 
 
 (* Still useful ?*)
 Lemma irrelevanceLift {l A F G Γ} (VΓ : [||-v Γ])
-  (VFG : [Γ ||-vS<l> F ≅ G | VΓ]) :
-  [Γ ,, F ||-vS<l> A | validSnoc VΓ VFG] ->
-  [Γ ,, G ||-vS<l> A | validSnoc VΓ (symmetry VFG)].
+  (VFG : [Γ ||-v<l> F ≅ G | VΓ]) :
+  [Γ ,, F ||-v<l> A | validSnoc VΓ VFG] ->
+  [Γ ,, G ||-v<l> A | validSnoc VΓ (symmetry VFG)].
 Proof.
   intros; eapply irrValidTy; tea; now eapply validSnoc.
 Qed.
@@ -269,27 +272,27 @@ Lemma irrValidTm {Γ0 Γ0' Γ1 Γ1' l l0 l1 A0 A0' A1 A1' t u}
   {VΓ0 : [||-v Γ0 ≅ Γ0']}
   {VΓ1 : [||-v Γ1 ≅ Γ1']}
   (VΓ01 : [||-v Γ0 ≅ Γ1])
-  (VA0 : [_ ||-vS<l0> A0 ≅ A0' | VΓ0])
-  (VA1 : [_ ||-vS<l1> A1 ≅ A1' | VΓ1]) :
-  [_ ||-vS<l> A0 ≅ A1 | VΓ01] ->
-  [_ ||-vS<l0> t ≅ u : _ | _ | VA0] ->
-  [_ ||-vS<l1> t ≅ u :  _ | _ | VA1].
+  (VA0 : [_ ||-v<l0> A0 ≅ A0' | VΓ0])
+  (VA1 : [_ ||-v<l1> A1 ≅ A1' | VΓ1]) :
+  [_ ||-v<l> A0 ≅ A1 | VΓ01] ->
+  [_ ||-v<l0> t ≅ u : _ | _ | VA0] ->
+  [_ ||-v<l1> t ≅ u :  _ | _ | VA1].
 Proof.
   intros VA Vt; constructor; intros.
   assert [VΓ0 | _ ||-v σ ≅ σ' : _ | wfΔ]
   by (eapply irrSubst; tea; now symmetry).
-  eapply SirrLRCum.
-  2: now unshelve now eapply SvalidTmExt.
-  eapply SvalidTyExt; tea.
+  eapply irrLRCum.
+  2: now unshelve now eapply validTmExt.
+  eapply validTyExt; tea.
   now eapply lrefl, convSubst.
 Qed.
 
 Lemma irrValidTmRfl {Γ Γ' l A A' B B' t u}
   {VΓ VΓ' : [||-v Γ ≅ Γ']}
-  {VA : [Γ ||-vS<l> A ≅ B | VΓ]}
-  {VA' : [Γ ||-vS<l> A' ≅ B' | VΓ']} :
+  {VA : [Γ ||-v<l> A ≅ B | VΓ]}
+  {VA' : [Γ ||-v<l> A' ≅ B' | VΓ']} :
   A = A' ->
-  [_ ||-vS<l> t ≅ u : _ | _ | VA] -> [_ ||-vS<l> t ≅ u : _ | _ | VA'].
+  [_ ||-v<l> t ≅ u : _ | _ | VA] -> [_ ||-v<l> t ≅ u : _ | _ | VA'].
 Proof.
   intros ?; subst.
   unshelve now eapply irrValidTm; eapply convValidTy; eapply lrefl.
@@ -297,34 +300,34 @@ Proof.
 Qed.
 
 
-Instance perValidTm {Γ Γ' l A A'} (VΓ : [||-v Γ ≅ Γ']) (VA : [_ ||-vS<l> A ≅ A' | VΓ]) :
-  PER (StermEqValidity _ _ _ _ _ VΓ VA).
+Instance perValidTm {Γ Γ' l A A'} (VΓ : [||-v Γ ≅ Γ']) (VA : [_ ||-v<l> A ≅ A' | VΓ]) :
+  PER (termEqValidity _ _ _ _ _ VΓ VA).
 Proof.
   constructor; red; intros; constructor; intros.
-  - eapply symLR, SirrLRConv.
-    2: (unshelve now eapply SvalidTmExt) ; tea; now symmetry.
-    eapply SvalidTyExt; tea; now eapply urefl.
-  - unshelve now etransitivity; eapply SirrLR; eapply SvalidTmExt.
+  - eapply symLR, irrLRConv.
+    2: (unshelve now eapply validTmExt) ; tea; now symmetry.
+    eapply validTyExt; tea; now eapply urefl.
+  - unshelve now etransitivity; eapply irrLR; eapply validTmExt.
     all: first [eassumption | now eapply lrefl].
 Qed.
 
 Lemma symValidTm {Γ Γ' l A A' t t'}
   {VΓ : [||-v Γ ≅ Γ']} (VΓ' : [||-v Γ' ≅ Γ])
-  {VA : [Γ ||-vS<l> A ≅ A' | VΓ]} (VA' : [_ ||-vS<l> A' ≅ A | VΓ']) :
-  [_ ||-vS<l> t ≅ t' : _ | _ | VA] -> [_ ||-vS<l> t' ≅ t : _ | _ | VA'].
+  {VA : [Γ ||-v<l> A ≅ A' | VΓ]} (VA' : [_ ||-v<l> A' ≅ A | VΓ']) :
+  [_ ||-v<l> t ≅ t' : _ | _ | VA] -> [_ ||-v<l> t' ≅ t : _ | _ | VA'].
 Proof. intros; symmetry; now eapply irrValidTm. Qed.
 
 Lemma symValidTm' {Γ Γ' l A A' t t'}
-  {VΓ : [||-v Γ ≅ Γ']} {VA : [_ ||-vS<l> A ≅ A' | VΓ]} :
-  [_ ||-vS<l> t ≅ t' : _ | _ | VA] -> [_ ||-vS<l> t' ≅ t : _ | _ | symValidTy' VA ].
+  {VΓ : [||-v Γ ≅ Γ']} {VA : [_ ||-v<l> A ≅ A' | VΓ]} :
+  [_ ||-v<l> t ≅ t' : _ | _ | VA] -> [_ ||-v<l> t' ≅ t : _ | _ | symValidTy' VA ].
 Proof. now apply symValidTm. Qed.
 
 Lemma transValidTm {Γ Γ' Γ'' l A A' A'' t t' t''}
   {VΓ : [||-v Γ ≅ Γ']} (VΓ' : [||-v Γ' ≅ Γ'']) (VΓ'' : [||-v Γ ≅ Γ''])
-  {VA : [Γ ||-vS<l> A ≅ A' | VΓ]} (VA' : [_ ||-vS<l> A' ≅ A'' | VΓ']) (VA'' : [_ ||-vS<l> A ≅ A'' | VΓ'']) :
-  [_ ||-vS<l> t ≅ t' : _ | _ | VA] ->
-  [_ ||-vS<l> t' ≅ t'' : _ | _ | VA'] ->
-  [_ ||-vS<l> t ≅ t'' : _ | _ | VA''].
+  {VA : [Γ ||-v<l> A ≅ A' | VΓ]} (VA' : [_ ||-v<l> A' ≅ A'' | VΓ']) (VA'' : [_ ||-v<l> A ≅ A'' | VΓ'']) :
+  [_ ||-v<l> t ≅ t' : _ | _ | VA] ->
+  [_ ||-v<l> t' ≅ t'' : _ | _ | VA'] ->
+  [_ ||-v<l> t ≅ t'' : _ | _ | VA''].
 Proof.
   intros; etransitivity; eapply irrValidTm.
   2,4: tea.
@@ -345,7 +348,7 @@ Proof.
     unshelve eexists (ih _ _ _ _ _ _ _ _ tl).
     1,2: red; intros; eauto.
     rewrite <- (eq1 var_zero); rewrite <- (eq2 var_zero).
-    eapply SirrLREq; tea; now rewrite eq1.
+    eapply irrLREq; tea; now rewrite eq1.
 Qed.
 
 End Irrelevances.
